lean/src/bpf/cfg.lean
@@ -33,6 +33,7 @@ inductive instr (α : Type*)
 | JMP64_X : JMP → reg → reg → α → α → instr
 | JMP64_K : JMP → reg → lsbvector 64 → α → α → instr
 | STX     : SIZE → reg → reg → lsbvector 64 → α → instr
+| LD_IMM  : reg → lsbvector 64 → α → instr
 | CALL    : BPF_FUNC → α → instr
 | Exit    : instr
 
@@ -47,6 +48,7 @@ private meta def to_pexpr' [has_to_pexpr α] : instr α → pexpr
 | (JMP64_X op r₁ r₂ if_true if_false)  := ``(JMP64_X %%op %%r₁ %%r₂ %%if_true %%if_false)
 | (JMP64_K op r₁ imm if_true if_false) := ``(JMP64_K %%op %%r₁ %%imm %%if_true %%if_false)
 | (STX size dst src off next)          := ``(STX %%size %%dst %%src %%off %%next)
+| (LD_IMM dst imm next)                := ``(LD_IMM %%dst %%imm %%next)
 | (CALL func next)                     := ``(CALL %%func %%next)
 | Exit                                 := ``(Exit)
 
@@ -60,6 +62,7 @@ private def repr' [has_repr α] : instr α → string
 | (JMP64_X op r1 r2 if_true if_false)  := "JMP64_X(" ++ repr op ++ ", " ++ repr r1 ++ ", " ++ repr r2 ++ ", " ++ repr if_true ++ ", " ++ repr if_false ++ ")"
 | (JMP64_K op r1 imm if_true if_false) := "JMP64_K(" ++ repr op ++ ", " ++ repr r1 ++ ", " ++ repr imm ++ ", " ++ repr if_true ++ ", " ++ repr if_false ++ ")"
 | (STX size dst src off next)          := "STX(" ++ repr size ++ ", " ++ repr dst ++ ", " ++ repr src ++ ", " ++ repr off ++ ", " ++ repr next ++ ")"
+| (LD_IMM dst imm next)                := "LD_IMM(" ++ repr dst ++ ", " ++ repr imm ++ ", " ++ repr next ++ ")"
 | (CALL func next)                     := "CALL(" ++ repr func ++ ", " ++ repr next ++ ")"
 | Exit                                 := "Exit()"
 
@@ -159,6 +162,9 @@ private def decode_flat_instr (cur : num) (pr : trie (instr pos_num)) : bpf.inst
 | (bpf.instr.STX op dst src off) :=
   let off64 := msb_imm16_sext_to_lsb_imm64 off in
   pr.kinsert cur.succ' (instr.STX op dst src off64 (cur + 1).succ')
+| (bpf.instr.LD_IMM dst imm64) :=
+  /- NB: cur + 2 because LD_IMM is two instructiosn (16 bytes) wide. -/
+  pr.kinsert cur.succ' (instr.LD_IMM dst imm64.reverse (cur + 2).succ')
 | (bpf.instr.CALL func) :=
   pr.kinsert cur.succ' (instr.CALL func (cur + 1).succ')
 | (bpf.instr.JMP64_X op dst src off) :=
